proof/refine/RISCV64/StateRelation.thy
@@ -142,13 +142,13 @@ definition arch_tcb_relation :: "Structures_A.arch_tcb \<Rightarrow> Structures_
 
 definition tcb_relation :: "Structures_A.tcb \<Rightarrow> Structures_H.tcb \<Rightarrow> bool" where
   "tcb_relation \<equiv> \<lambda>tcb tcb'.
-     tcb_fault_handler tcb = to_bl (tcbFaultHandler tcb')
-   \<and> tcb_ipc_buffer tcb = tcbIPCBuffer tcb'
+     tcb_ipc_buffer tcb = tcbIPCBuffer tcb'
    \<and> arch_tcb_relation (tcb_arch tcb) (tcbArch tcb')
    \<and> thread_state_relation (tcb_state tcb) (tcbState tcb')
    \<and> fault_rel_optionation (tcb_fault tcb) (tcbFault tcb')
    \<and> cap_relation (tcb_ctable tcb) (cteCap (tcbCTable tcb'))
    \<and> cap_relation (tcb_vtable tcb) (cteCap (tcbVTable tcb'))
+   \<and> cap_relation (tcb_fault_handler tcb) (cteCap (tcbFaultHandler tcb'))
    \<and> cap_relation (tcb_reply tcb) (cteCap (tcbReply tcb'))
    \<and> cap_relation (tcb_caller tcb) (cteCap (tcbCaller tcb'))
    \<and> cap_relation (tcb_ipcframe tcb) (cteCap (tcbIPCBufferFrame tcb'))
